introduced delete

Main.lean
@@ -21,18 +21,23 @@ def equiv (jd: JDB) (sd: SDB) : Prop :=
 
 inductive JQuery where
   | find : (Juser → Bool) → JQuery
+  | delete : (Juser → Bool) → JQuery
 
 inductive SQuery where
   | select : (Juser → Bool) → SQuery
+  | drop : (Juser → Bool) → SQuery
 
 def jqueryToSquery : JQuery → SQuery
   | .find p => .select p
+  | .delete p => .drop p
 
 def eval_jquery (jd : JDB) : JQuery → JDB
   | .find p => jd.filter p
+  | .delete p => jd.filter (fun u => ¬ p u)
 
 def eval_squery (sd : SDB) : SQuery → SDB
   | .select p => sd.filter (fun r => p {name := r.1, age := r.2})
+  | .drop p => sd.filter (fun r => ¬ p {name := r.1, age := r.2})
 
 theorem jdbToSdb_filter (jd: JDB) (p: Juser → Bool) :
     jdbToSdb (jd.filter p) =
@@ -62,6 +67,27 @@ theorem sdbToJdb_filter (sd: SDB) (p: Juser → Bool) :
           · rename_i h
             simp [ih]
 
+theorem delete_equiv1 (jd : JDB) (sd : SDB) (p : Juser → Bool) (h : equiv jd sd) :
+    jdbToSdb (eval_jquery jd (.delete p)) = eval_squery sd (.drop p) := by
+  rcases h with ⟨h_to_sdb, _⟩
+  simp [eval_jquery, eval_squery]
+  rw [jdbToSdb_filter jd (fun u => !(p u))]
+  rw [h_to_sdb]
+
+theorem delete_equiv2 (jd : JDB) (sd : SDB) (p : Juser → Bool) (h : equiv jd sd) :
+    sdbToJdb (eval_squery sd (.drop p)) = eval_jquery jd (.delete p) := by
+  rcases h with ⟨_, h_to_jdb⟩
+  simp [eval_jquery, eval_squery]
+  rw [sdbToJdb_filter sd (fun u => !(p u))]
+  rw [h_to_jdb]
+
+-- The main result for Delete
+theorem delete_equiv (jd : JDB) (sd : SDB) (p : Juser → Bool) (h : equiv jd sd) :
+    equiv (eval_jquery jd (.delete p)) (eval_squery sd (.drop p)) := by
+  constructor
+  · exact delete_equiv1 jd sd p h
+  · exact delete_equiv2 jd sd p h
+
 theorem query_equiv1 (jd : JDB) (sd : SDB) (jq : JQuery) (h : equiv jd sd) :
     jdbToSdb (eval_jquery jd jq) = eval_squery sd (jqueryToSquery jq) := by
   rcases h with ⟨h_to_sdb, _⟩
@@ -69,15 +95,23 @@ theorem query_equiv1 (jd : JDB) (sd : SDB) (jq : JQuery) (h : equiv jd sd) :
   | find p =>
       simp [eval_jquery, eval_squery, jqueryToSquery]
       rw [jdbToSdb_filter, h_to_sdb]
+  | delete p =>
+      simp [eval_jquery, eval_squery, jqueryToSquery]
+      rw [jdbToSdb_filter jd (fun u => !(p u))]
+      rw [h_to_sdb]
 
 theorem query_equiv2 (jd : JDB) (sd : SDB) (jq : JQuery) (h : equiv jd sd) :
     sdbToJdb (eval_squery sd (jqueryToSquery jq)) = (eval_jquery jd jq) := by
   rcases h with ⟨_, h_to_jdb⟩
   cases jq with
   | find p =>
-    simp [eval_jquery, eval_squery, jqueryToSquery]
-    -- We use the lemma to show that filtering tuples is same as filtering Users
-    rw [sdbToJdb_filter, h_to_jdb]
+      simp [eval_jquery, eval_squery, jqueryToSquery]
+      -- We use the lemma to show that filtering tuples is same as filtering Users
+      rw [sdbToJdb_filter, h_to_jdb]
+  | delete p =>
+      simp [eval_jquery, eval_squery, jqueryToSquery]
+      rw [sdbToJdb_filter sd (fun u => !(p u))]
+      rw [h_to_jdb]
 
 theorem query_equiv (jd : JDB) (sd : SDB) (jq : JQuery) (h : equiv jd sd) :
     equiv (eval_jquery jd jq) (eval_squery sd (jqueryToSquery jq)) := by
